open import Prelude

module Language.STLC.Term where

open import Language.Type

infixr 5 Æ›_
infixl 7 _Â·_
infixr 8 âŸª_âŸ«_ âŸ¨_âŸ©_
infixr 9 `_ -- #_

data Tm (Î“ : Ty â†’ Type) : Ty â†’ Type

private
  variable
    A B C          : Ty
    Î“ Î” Î          : Ty â†’ Type
    t u v tâ€² uâ€² vâ€² : Tm Î“ A

data Tm Î“ where
  `_
    : (x : Î“ A)
    â†’ Tm Î“ A
  _Â·_
    : (t : Tm Î“ (A â‡’ B)) (u : Tm Î“ A)
    â†’ Tm Î“ B
  Æ›_
    : Tm (Î“ â–· A) B
    â†’ Tm Î“ (A â‡’ B)

Ren : (Î“ Î” : Ty â†’ Type) â†’ Type
Ren Î“ Î” = âˆ€ {A} â†’ Î” A â†’ Î“ A

_â¨ŸÊ³_ : Ren Î“ Î” â†’ Ren Î” Î â†’ Ren Î“ Î
Ï â¨ŸÊ³ Ïâ€² = Ï âˆ˜ Ïâ€² 

ext : Ren Î“ Î” â†’ Ren (Î“ â–· A) (Î” â–· A)
ext Ï Z     = Z
ext Ï (S x) = S Ï x

-- renaming is map:
-- (Ï : âˆ€ {A} â†’ Î” A â†’ Î“ A)
-- -----------------------
-- âˆ€ {A} â†’ Tm Î” A â†’ Tm Î“ A
âŸ¨_âŸ©_ : Ren Î“ Î” â†’ Tm Î” A â†’ Tm Î“ A
âŸ¨ Ï âŸ© (` x)   = ` Ï x
âŸ¨ Ï âŸ© (t Â· u) = âŸ¨ Ï âŸ© t Â· âŸ¨ Ï âŸ© u
âŸ¨ Ï âŸ© (Æ› t)   = Æ› âŸ¨ ext Ï âŸ© t

postulate
-- map id = id
  ren-id
    : (t : Tm Î“ A)
    â†’ âŸ¨ (Î» x â†’ x) âŸ© t â‰¡ t
-- map (f âˆ˜ g) = map f âˆ˜ map g
  ren-comp
    : (Ï : Ren Î“ Î”) (Ïâ€² : Ren Î” Î)
    â†’ (t : Tm Î A)
    â†’ âŸ¨ Ï âˆ˜ Ïâ€² âŸ© t â‰¡ âŸ¨ Ï âŸ© âŸ¨ Ïâ€² âŸ© t

Sub : (Î“ Î” : Ty â†’ Type) â†’ Type
Sub Î“ Î” = {A : Ty} â†’ Î” A â†’ Tm Î“ A

exts : Sub Î“ Î” â†’ Sub (Î“ â–· A) (Î” â–· A)
exts Ïƒ Z     = ` Z
exts Ïƒ (S x) = âŸ¨ S_ âŸ© Ïƒ x

âŸª_âŸ«_ : Sub Î“ Î” â†’ (Tm Î” A â†’ Tm Î“ A)
âŸª Ïƒ âŸ« (` x)   = Ïƒ x
âŸª Ïƒ âŸ« (t Â· u) = âŸª Ïƒ âŸ« t Â· âŸª Ïƒ âŸ« u
âŸª Ïƒ âŸ« (Æ› t)   = Æ› âŸª exts Ïƒ âŸ« t

_âˆ·_ : Sub Î“ Î” â†’ Tm Î“ A â†’ Sub Î“ (Î” â–· A)
(Ïƒ âˆ· t) Z     = t
(Ïƒ âˆ· t) (S x) = Ïƒ x

[_]_
  : Tm Î“ B
  â†’ Tm (Î“ â–· B) A 
  â†’ Tm Î“ A
[ u ] t = âŸª `_ âˆ· u âŸ« t

_â¨Ÿ_
  : {Z : Ty â†’ Type}
  â†’ Sub Î“ Î” â†’ Sub Î” Z â†’ Sub Î“ Z
(Ïƒ â¨Ÿ Ïƒâ€²) x = âŸª Ïƒ âŸ« Ïƒâ€² x

â‡‘_ : Ren Î“ Î” â†’ Sub Î“ Î”
(â‡‘ Ï) x = ` Ï x

subst-idR : (Ïƒ : Sub Î“ Î”)
  â†’ (x : Î” A)
  â†’ âŸª Ïƒ âŸ« (` x) â‰¡ Ïƒ x
subst-idR Ïƒ x = refl

exts-ids=ids
  : (x : (Î“ â–· B) A)
  â†’ exts `_ x â‰¡ ` x
exts-ids=ids Z     = refl
exts-ids=ids (S x) = refl

subst-idL : (t : Tm Î“ A)
  â†’ âŸª `_ âŸ« t â‰¡ t
subst-idL (` x)   = refl
subst-idL (t Â· u) = congâ‚‚ _Â·_ (subst-idL t) (subst-idL u)
subst-idL (Æ› t)   = cong Æ›_ (
  âŸª exts `_ âŸ« t
    â‰¡[ i ]âŸ¨ âŸª (Î» x â†’ exts-ids=ids x i) âŸ« t âŸ©
  âŸª `_ âŸ« t
    â‰¡âŸ¨ subst-idL t âŸ©
  t âˆ)
  where open â‰¡-Reasoning

-- tedious to prove
postulate
  ren-exts : (Ïƒ : Sub Î“ Î”)
    â†’ (t : Tm Î” A)
    â†’ âŸª exts {A = B} Ïƒ âŸ« âŸ¨ S_ âŸ© t â‰¡ âŸ¨ S_ âŸ© âŸª Ïƒ âŸ« t

exts-comp : {Z : Ty â†’ Type}
  â†’ (Ïƒ : Sub Î“ Î”) (Ïƒâ€² : Sub Î” Z)
  â†’ (x : (Z â–· B) A)
  â†’ (exts Ïƒ â¨Ÿ exts Ïƒâ€²) x â‰¡ exts (Ïƒ â¨Ÿ Ïƒâ€²) x
exts-comp Ïƒ Ïƒâ€² Z     = refl
exts-comp Ïƒ Ïƒâ€² (S x) = begin
  (exts Ïƒ â¨Ÿ exts Ïƒâ€²) (S x)
    â‰¡âŸ¨ refl âŸ©
  âŸª exts Ïƒ âŸ« âŸ¨ S_ âŸ© (Ïƒâ€² x)
    â‰¡âŸ¨ ren-exts Ïƒ (Ïƒâ€² x) âŸ©
  âŸ¨ S_ âŸ© âŸª Ïƒ âŸ« (Ïƒâ€² x)
    â‰¡âŸ¨ refl âŸ©
  exts (Ïƒ â¨Ÿ Ïƒâ€²) (S x) âˆ
  where open â‰¡-Reasoning

subst-assoc
  : {Z : Ty â†’ Type}
  â†’ (Ïƒ : Sub Î“ Î”) (Ïƒâ€² : Sub Î” Z)
  â†’ (t : Tm Z A)
  â†’ âŸª Ïƒ âŸ« âŸª Ïƒâ€² âŸ« t â‰¡ âŸª Ïƒ â¨Ÿ Ïƒâ€² âŸ« t
subst-assoc Ïƒ Ïƒâ€² (` x)   = refl
subst-assoc Ïƒ Ïƒâ€² (t Â· u) = congâ‚‚ _Â·_
  (subst-assoc Ïƒ Ïƒâ€² t) (subst-assoc Ïƒ Ïƒâ€² u)
subst-assoc Ïƒ Ïƒâ€² (Æ› t)   = cong Æ›_
  (âŸª exts Ïƒ âŸ« âŸª exts Ïƒâ€² âŸ« t
    â‰¡âŸ¨ subst-assoc (exts Ïƒ) (exts Ïƒâ€²) t âŸ©
  âŸª exts Ïƒ â¨Ÿ exts Ïƒâ€² âŸ« t
    â‰¡[ i ]âŸ¨ âŸª (Î» x â†’ exts-comp Ïƒ Ïƒâ€² x i) âŸ« t âŸ©
   âŸª exts (Ïƒ â¨Ÿ Ïƒâ€²) âŸ« t âˆ)
  where open â‰¡-Reasoning

infix 3 _-â†’_
data _-â†’_ {Î“} : (t u : Tm Î“ A) â†’ ğ“¤â‚€ Ì‡ where
  Î²-Æ›Â·
    : (Æ› t) Â· u -â†’ [ u ] t
  Î¾-Æ›
    :   t -â†’ tâ€²
    â†’ Æ› t -â†’ Æ› tâ€²    
  Î¾-Â·â‚—
    :     t -â†’ tâ€²
      ---------------
    â†’ t Â· u -â†’ tâ€² Â· u
  Î¾-Â·áµ£
    :     u -â†’ uâ€²
      ---------------
    â†’ t Â· u -â†’ t Â· uâ€²

data _-â† _ {Î“ A} : (t u : Tm Î“ A) â†’ ğ“¤â‚€ Ì‡ where
  _âˆ : (t : Tm Î“ A)
    â†’ t -â†  t
    
  _-â†’âŸ¨_âŸ©_
    : âˆ€ t   
    â†’ t -â†’ u
    â†’ u -â†  v
      -------
    â†’ t -â†  v

infix  2 _-â† _ 
infixr 2 _-â†’âŸ¨_âŸ©_
infix 3 _âˆ

_-â† âŸ¨_âŸ©_
  : (t : Tm Î“ A)
  â†’ t -â†  u â†’ u -â†  v
  -----------------
  â†’ t -â†  v
t -â† âŸ¨ t âˆ         âŸ© w = w
t -â† âŸ¨ t -â†’âŸ¨ x âŸ© r âŸ© w = t -â†’âŸ¨ x âŸ© _ -â† âŸ¨ r âŸ© w

infixr 2 _-â† âŸ¨_âŸ©_
